RocqOfRust/revm/revm_interpreter/instructions/simulate/control/jumpdest.v
@@ -3,7 +3,7 @@ Require Import alloy_primitives.bytes.simulate.mod.
 Require Import alloy_primitives.links.aliases.
 Require Import core.links.array.
 Require Import revm.revm_interpreter.gas.simulate.constants.
-Require Import revm.revm_interpreter.instructions.links.control.jumpdest_or_nop.
+Require Import revm.revm_interpreter.instructions.links.control.jumpdest.
 Require Import revm.revm_interpreter.instructions.simulate.macros.
 Require Import revm.revm_interpreter.links.gas.
 Require Import revm.revm_interpreter.links.instruction_result.
@@ -18,15 +18,15 @@ Require Import ruint.simulate.cmp.
 Require Import ruint.simulate.from.
 Require Import ruint.simulate.lib.
 
-Definition jumpdest_or_nop
+Definition jumpdest
     {WIRE : Set} `{Link WIRE}
     {WIRE_types : InterpreterTypes.Types.t} `{InterpreterTypes.Types.AreLinks WIRE_types}
     {IInterpreterTypes : InterpreterTypes.C WIRE_types}
     (interpreter : Interpreter.t WIRE WIRE_types) :
     Interpreter.t WIRE WIRE_types :=
-  gas_macro interpreter constants.JUMPDEST id id.
+  interpreter.
 
-Lemma jumpdest_or_nop_eq
+Lemma jumpdest_eq
     {WIRE H : Set} `{Link WIRE} `{Link H}
     {WIRE_types : InterpreterTypes.Types.t} `{InterpreterTypes.Types.AreLinks WIRE_types}
     (run_InterpreterTypes_for_WIRE : InterpreterTypes.Run WIRE WIRE_types)
@@ -37,18 +37,20 @@ Lemma jumpdest_or_nop_eq
     (_host : H) :
   let ref_interpreter := make_ref 0 in
   let ref_host := make_ref (A := H) 1 in
+  let context := {|
+    instruction_context.InstructionContext.interpreter := ref_interpreter;
+    instruction_context.InstructionContext.host := ref_host;
+  |} in
   {{
     SimulateM.eval_f
-      (run_jumpdest_or_nop run_InterpreterTypes_for_WIRE ref_interpreter ref_host)
+      (run_jumpdest run_InterpreterTypes_for_WIRE context)
       ([interpreter; _host]%stack) 🌲
     (
       Output.Success tt,
-      [jumpdest_or_nop interpreter; _host]%stack
+      [jumpdest interpreter; _host]%stack
     )
   }}.
 Proof.
-  intros.
-  with_strategy transparent [run_jumpdest_or_nop] unfold jumpdest_or_nop, run_jumpdest_or_nop; cbn.
-  gas_macro_eq idtac.
+  with_strategy transparent [run_jumpdest] unfold jumpdest, run_jumpdest; cbn.
   s.
 Qed.
