RocqOfRust/revm/revm_interpreter/instructions/links/control/jump_inner.v
@@ -36,9 +36,10 @@ Instance run_jump_inner
     unit.
 Proof.
   constructor.
-  destruct run_InterpreterTypes_for_WIRE.
+  destruct run_InterpreterTypes_for_WIRE eqn:?.
   destruct run_LoopControl_for_Control.
   destruct run_Jumps_for_Bytecode.
   run_symbolic.
+  all: eapply (@Impl_Interpreter.run_halt WIRE H WIRE_types H0 run_InterpreterTypes_for_WIRE).
 Defined.
 Global Opaque run_jump_inner.
