RocqOfRust/revm/revm_interpreter/simulate/interpreter_action.v
@@ -1,0 +1,39 @@
+Require Import simulate.RocqOfRust.
+Require Import alloy_primitives.bytes.links.mod.
+Require Import alloy_primitives.bytes.simulate.mod.
+Require Import revm.revm_interpreter.links.gas.
+Require Import revm.revm_interpreter.links.interpreter_action.
+Require Import revm.revm_interpreter.links.interpreter_InterpreterResult.
+Require Import revm.revm_interpreter.links.instruction_result.
+
+Definition new_return
+    (result : InstructionResult.t)
+    (output : Bytes.t)
+    (gas : Gas.t) :
+    InterpreterAction.t :=
+  InterpreterAction.Return {|
+    InterpreterResult.result := result;
+    InterpreterResult.output := output;
+    InterpreterResult.gas := gas;
+  |}.
+
+Lemma new_return_eq
+    (result : InstructionResult.t)
+    (output : Bytes.t)
+    (gas : Gas.t)
+    (stack : Stack.t) :
+  {{
+    SimulateM.eval_f
+      (Impl_InterpreterAction.run_new_return result output gas)
+      stack 🌲
+    (
+      Output.Success (new_return result output gas),
+      stack
+    )
+  }}.
+Proof.
+  with_strategy transparent [Impl_InterpreterAction.run_new_return]
+    unfold new_return, Impl_InterpreterAction.run_new_return.
+  cbn.
+  s.
+Qed.
